@prefix : <https://purl.org/homerent/> .
@prefix dc: <http://purl.org/dc/elements/1.1/> .
@prefix gn: <https://www.geonames.org/ontology#> .
@prefix dct: <http://purl.org/dc/terms/> .
@prefix owl: <http://www.w3.org/2002/07/owl#> .
@prefix rdf: <http://www.w3.org/1999/02/22-rdf-syntax-ns#> .
@prefix xml: <http://www.w3.org/XML/1998/namespace> .
@prefix xsd: <http://www.w3.org/2001/XMLSchema#> .
@prefix foaf: <http://xmlns.com/foaf/0.1/> .
@prefix rdfs: <http://www.w3.org/2000/01/rdf-schema#> .
@prefix vann: <http://purl.org/vocab/vann/> .
@prefix schema: <http://schema.org/> .
@base <https://purl.org/homerent/> .

<https://purl.org/homerent/> rdf:type owl:Ontology ;
                              owl:imports <http://purl.org/goodrelations/v1> ;
                              dc:rights "This ontology is licensed under MIT" ;
                              dct:creator [ rdf:type foaf:Person ;
                                            foaf:name "Andrea" ;
                                            foaf:surname "Giulianelli"
                                          ] ;
                              dct:description """
                                L'ontologia di HomeRent ha l'obiettivo principale di modellare il dominio degli affitti di appartamenti.
                              """@it ,
                                              """
                                The HomeRent ontology has the main goal of modeling the apartment rental domain.
                              """@en ;
                              dct:license <https://opensource.org/license/mit/> ;
                              dct:title "HomeRent Ontology" ;
                              vann:preferredNamespacePrefix "hr" ;
                              rdfs:label "HomeRent ontology"@en ;
                              owl:versionInfo "1.0.0" .

#################################################################
#    Annotation properties
#################################################################

###  http://purl.org/dc/terms/creator
dct:creator rdf:type owl:AnnotationProperty .


###  http://purl.org/dc/terms/description
dct:description rdf:type owl:AnnotationProperty .


###  http://purl.org/dc/terms/title
dct:title rdf:type owl:AnnotationProperty .


###  http://purl.org/vocab/vann/preferredNamespacePrefix
vann:preferredNamespacePrefix rdf:type owl:AnnotationProperty .


###  http://xmlns.com/foaf/0.1/name
foaf:name rdf:type owl:AnnotationProperty .


###  http://xmlns.com/foaf/0.1/surname
foaf:surname rdf:type owl:AnnotationProperty .


#################################################################
#    Object Properties
#################################################################

###  http://purl.org/goodrelations/v1#includes
<http://purl.org/goodrelations/v1#includes> owl:inverseOf :isApartmentIncluded .


###  http://purl.org/goodrelations/v1#offers
<http://purl.org/goodrelations/v1#offers> owl:inverseOf :isOfferedBy .


###  https://purl.org/homerent/geoName
:geoName rdf:type owl:ObjectProperty ,
                  owl:FunctionalProperty ;
         rdfs:domain schema:PostalAddress ;
         rdfs:range gn:Feature ;
         rdfs:comment "Questa proprietà permette di collegare un indirizzo alla posizione esatta espressa come feature geoname."@it ,
                      "This property allows to link an address to the exact location expressed as a geoname feature."@en ;
         rdfs:isDefinedBy <https://purl.org/homerent/> ;
         rdfs:label "geo name"@en .


###  https://purl.org/homerent/hasAppliance
:hasAppliance rdf:type owl:ObjectProperty ;
              rdfs:subPropertyOf :hasFeature ;
              rdfs:range :Appliance ;
              owl:propertyDisjointWith :hasService ;
              rdfs:comment "Questa proprietà permette di mettere in relazione l'appartamento con gli elettrodomestici presenti al suo interno."@it ,
                           "This property allows to link an apartment to the appliance inside it."@en ;
              rdfs:isDefinedBy <https://purl.org/homerent/> ;
              rdfs:label "ha elettrodomestico"@it ,
                         "has appliance"@en .


###  https://purl.org/homerent/hasExpense
:hasExpense rdf:type owl:ObjectProperty ;
            owl:propertyChainAxiom ( <http://purl.org/goodrelations/v1#hasPriceSpecification>
                                     :priceComponent
                                   ) ;
            rdfs:comment "Questa proprietà lega l'appartamento alle sue spese."@it ,
                         "This property links the apartment to its expenses."@en ;
            rdfs:isDefinedBy <https://purl.org/homerent/> ;
            rdfs:label "ha spesa"@it ,
                       "has expense"@en .


###  https://purl.org/homerent/hasFeature
:hasFeature rdf:type owl:ObjectProperty ;
            rdfs:domain schema:Apartment ;
            rdfs:range :Feature ;
            rdfs:comment "Questa proprietà collega un appartamento alle funzionalità messe a disposizione."@it ,
                         "This property links an apartment to its features."@en ;
            rdfs:isDefinedBy <https://purl.org/homerent/> ;
            rdfs:label "ha funzionalità"@it ,
                       "has feature"@en .


###  https://purl.org/homerent/hasFloorType
:hasFloorType rdf:type owl:ObjectProperty ;
              rdfs:domain schema:Apartment ;
              rdfs:range :FloorType ;
              rdfs:comment "Questa proprietà è necessaria per specificare il tipo di pavimento di un appartamento."@it ,
                           "This property is necessary to specify the floor type of an apartment."@en ;
              rdfs:isDefinedBy <https://purl.org/homerent/> ;
              rdfs:label "floor type"@en ,
                         "tipo di pavimento"@it .


###  https://purl.org/homerent/hasGeneratedInterest
:hasGeneratedInterest rdf:type owl:ObjectProperty ;
                      owl:inverseOf :refersRentAd ;
                      rdfs:comment "Questa proprietà collega un annuncio di affitto all'interesse che genera."@it ,
                                   "This property links a rental ad to the interest that it generates."@en ;
                      rdfs:isDefinedBy <https://purl.org/homerent/> ;
                      rdfs:label "ha generato interesse"@it ,
                                 "has generated interest"@en .


###  https://purl.org/homerent/hasInterestIn
:hasInterestIn rdf:type owl:ObjectProperty ;
               owl:inverseOf :isOfInterestTo ;
               rdfs:comment "Questa proprietà è necessaria per connettere le persone con i loro interessi."@it ,
                            "This property is needed to connect people to their interests."@en ;
               rdfs:isDefinedBy <https://purl.org/homerent/> ;
               rdfs:label "has interest in"@en ,
                          "è interessato a"@it .


###  https://purl.org/homerent/hasService
:hasService rdf:type owl:ObjectProperty ;
            rdfs:subPropertyOf :hasFeature ;
            rdfs:range :Service ;
            rdfs:comment "Questa proprietà permette di mettere in relazione un appartamento con i servizi messi a disposizione."@it ,
                         "This property allows to link an apartment with the services that are provided."@en ;
            rdfs:isDefinedBy <https://purl.org/homerent/> ;
            rdfs:label "fornisce servizio"@it ,
                       "has service"@en .


###  https://purl.org/homerent/isApartmentIncluded
:isApartmentIncluded rdf:type owl:ObjectProperty ;
                     rdfs:comment "Questa è la proprietà inversa di gr:includes e modella il fatto che un appartamento è incluso in un annuncio di affitto."@it ,
                                  "This is the inverse property of gr:includes and models the fact that an apartment is included in a rental ad."@en ;
                     rdfs:isDefinedBy <https://purl.org/homerent/> ;
                     rdfs:label "is apartment included in"@en ,
                                "l'appartamento è incluso nel"@it .


###  https://purl.org/homerent/isAvailableFor
:isAvailableFor rdf:type owl:ObjectProperty ;
                rdfs:domain schema:Apartment ;
                rdfs:range <http://purl.org/goodrelations/v1#QuantitativeValueFloat> ;
                rdfs:comment "Questa proprietà permette di specificare per quanto tempo l'appartamento è disponibile."@it ,
                             "This property allows you to specify how long the apartment is available."@en ;
                rdfs:isDefinedBy <https://purl.org/homerent/> ;
                rdfs:label "is available for"@en ,
                           "è disponibile per"@it .


###  https://purl.org/homerent/isOfInterestTo
:isOfInterestTo rdf:type owl:ObjectProperty ,
                         owl:FunctionalProperty ;
                rdfs:domain :RentalAdInterest ;
                rdfs:range schema:Person ;
                rdfs:comment "Questa proprietà connette un interesse alla persona interessata."@it ,
                             "This property connects an interest to the interested person."@en ;
                rdfs:isDefinedBy <https://purl.org/homerent/> ;
                rdfs:label "is of interest to"@en ,
                           "è di interesse per"@it .


###  https://purl.org/homerent/isOfferedBy
:isOfferedBy rdf:type owl:ObjectProperty ,
                      owl:FunctionalProperty ;
             rdfs:domain :RentalAd ;
             rdfs:range <http://purl.org/goodrelations/v1#BusinessEntity> ;
             rdfs:comment "Questa proprietà è l'inverso di gr:offers e modella che un annuncio di affitto è offerto da una entità di business."@it ,
                          "This property is the inverse of gr:offer modelling the fact that a rental ad is offered by a business entity."@en ;
             rdfs:isDefinedBy <https://purl.org/homerent/> ;
             rdfs:label "is offered by"@en ,
                        "offerto da"@it .


###  https://purl.org/homerent/isPossibleToReach
:isPossibleToReach rdf:type owl:ObjectProperty ;
                   owl:inverseOf :reachableFrom ;
                   rdfs:domain schema:Apartment ;
                   rdfs:range :StrategicPoint ;
                   rdfs:comment "Questa proprietà collega un appartamento con i punti strategici che si possono raggiungere."@it ,
                                "This property connects an apartment to strategic points that can be reached."@en ;
                   rdfs:isDefinedBy <https://purl.org/homerent/> ;
                   rdfs:label "is possible to reach"@en ,
                              "è possibile raggiungere"@it .


###  https://purl.org/homerent/isReachable
:isReachable rdf:type owl:ObjectProperty ;
             owl:propertyChainAxiom ( :isPossibleToReach
                                      :strategicPointRefersTo
                                    ) .


###  https://purl.org/homerent/priceComponent
:priceComponent rdf:type owl:ObjectProperty ;
                rdfs:domain :CompoundPrice ;
                rdfs:range <http://purl.org/goodrelations/v1#UnitPriceSpecification> ;
                rdfs:comment "Questa proprietà permette di specificare i componenti del prezzo."@it ,
                             "This property allows to specify the price components."@en ;
                rdfs:isDefinedBy <https://purl.org/homerent/> ;
                rdfs:label "componente del prezzo"@it ,
                           "price component"@en .


###  https://purl.org/homerent/reachableFrom
:reachableFrom rdf:type owl:ObjectProperty ,
                        owl:FunctionalProperty ;
               rdfs:comment "Questa proprietà indica da quale appartamento il punto strategico è raggiungibile."@it ,
                            "This property indicate from which apartment the stratetic point can be reached."@en ;
               rdfs:isDefinedBy <https://purl.org/homerent/> ;
               rdfs:label "raggiungibile da"@it ,
                          "reachable from"@en .


###  https://purl.org/homerent/refersRentAd
:refersRentAd rdf:type owl:ObjectProperty ,
                       owl:FunctionalProperty ;
              rdfs:domain :RentalAdInterest ;
              rdfs:range :RentalAd ;
              rdfs:comment "Questa proprietà è necessaria per collegare un interesse all'annuncio di affitto a cui si riferisce."@it ,
                           "This property is required to link an interest to the rental ad to which it refers."@en ;
              rdfs:isDefinedBy <https://purl.org/homerent/> ;
              rdfs:label "refers rent ad"@en ,
                         "riferito al seguente annuncio di affitto"@it .


###  https://purl.org/homerent/strategicPointRefersTo
:strategicPointRefersTo rdf:type owl:ObjectProperty ,
                                 owl:FunctionalProperty ;
                        rdfs:domain :StrategicPoint ;
                        rdfs:range :ReachablePlace ;
                        rdfs:comment "Questa proprietà permette di mettere in relazione il punto strategico al luogo raggiungibile."@it ,
                                     "This property allows to link the strategic point to the reachable place."@en ;
                        rdfs:isDefinedBy <https://purl.org/homerent/> ;
                        rdfs:label "il punto strategico si riferisce a"@it ,
                                   "strategic point refers to"@en .


#################################################################
#    Data properties
#################################################################

###  http://schema.org/startDate
schema:startDate rdf:type owl:DatatypeProperty ;
                 owl:equivalentProperty :interestDateTime .


###  https://purl.org/homerent/busLine
:busLine rdf:type owl:DatatypeProperty ;
         rdfs:range xsd:string ;
         rdfs:comment "Questa proprietà permette di specificare la linea del bus della fermata."@it ,
                      "This property allows to specify the bus line of the bus stop."@en ;
         rdfs:isDefinedBy <https://purl.org/homerent/> ;
         rdfs:label "bus line"@en ,
                    "linea del bus"@it .


###  https://purl.org/homerent/distanceInKm
:distanceInKm rdf:type owl:DatatypeProperty ,
                       owl:FunctionalProperty ;
              rdfs:range xsd:float ;
              rdfs:comment "Questa proprietà permette di specificare la distanza in km da un punto strategico."@it ,
                           "This property allows to specify the distance from a Strategic point in km."@en ;
              rdfs:isDefinedBy <https://purl.org/homerent/> ;
              rdfs:label "distance in km"@en ,
                         "distanza in km"@it .


###  https://purl.org/homerent/floorDescription
:floorDescription rdf:type owl:DatatypeProperty ;
                  rdfs:range xsd:string ;
                  rdfs:comment "Questa proprietà permette di descrivere il tipo di pavimentazione presente in un appartamento."@it ,
                               "This property allows to describe the type of the floor that is inside an apartment."@en ;
                  rdfs:isDefinedBy <https://purl.org/homerent/> ;
                  rdfs:label "descrizione del tipo di pavimentazione"@it ,
                             "floor description"@en .


###  https://purl.org/homerent/interestDateTime
:interestDateTime rdf:type owl:DatatypeProperty ;
                  rdfs:subPropertyOf owl:topDataProperty ;
                  rdf:type owl:FunctionalProperty ;
                  rdfs:comment "Questa proprietà modella la data e l'ora di un interesse ad annuncio di affitto."@it ,
                               "This property models the date and the time of the interest in a rental ad."@en ;
                  rdfs:isDefinedBy <https://purl.org/homerent/> ;
                  rdfs:label "data e ora dell'interesse"@it ,
                             "interest date time"@en .


###  https://purl.org/homerent/isAvailableFrom
:isAvailableFrom rdf:type owl:DatatypeProperty ,
                          owl:FunctionalProperty ;
                 rdfs:domain schema:Apartment ;
                 rdfs:range xsd:dateTime ;
                 rdfs:comment "Questa proprietà è necessaria per indicare la data di inizio disponibilità di un appartamento."@it ,
                              "This property is required to specify the availability start date of an apartment."@en ;
                 rdfs:isDefinedBy <https://purl.org/homerent/> ;
                 rdfs:label "is available from"@en ,
                            "è disponibile da"@it .


###  https://purl.org/homerent/isFeatureUsageShared
:isFeatureUsageShared rdf:type owl:DatatypeProperty ,
                               owl:FunctionalProperty ;
                      rdfs:range xsd:boolean ;
                      rdfs:comment "Questa proprietà indica se l'utilizzo della funzionalità è condiviso oppure no."@it ,
                                   "This property specifies if the usage of the feature is shared or not."@en ;
                      rdfs:isDefinedBy <https://purl.org/homerent/> ;
                      rdfs:label "is feature usage shared"@en ,
                                 "l'utilizzo è condiviso?"@it .


###  https://purl.org/homerent/isFurnished
:isFurnished rdf:type owl:DatatypeProperty ,
                      owl:FunctionalProperty ;
             rdfs:domain schema:Apartment ;
             rdfs:range xsd:boolean ;
             rdfs:comment "Questa proprietà indica se un appartamento è arredato."@it ,
                          "This property indicates if an apartment is furnished."@en ;
             rdfs:isDefinedBy <https://purl.org/homerent/> ;
             rdfs:label "is furnished"@en ,
                        "è arredata"@it .


###  https://purl.org/homerent/isReadyToLive
:isReadyToLive rdf:type owl:DatatypeProperty ,
                        owl:FunctionalProperty ;
               rdfs:domain schema:Apartment ;
               rdfs:range xsd:boolean ;
               rdfs:comment "Questa proprietà indica se un appartamento è pronto per abitarci."@it ,
                            "This property indicate if an apartment is ready to live in."@en ;
               rdfs:isDefinedBy <https://purl.org/homerent/> ;
               rdfs:label "is ready to live"@en ,
                          "è pronta per viverci"@it .


###  https://purl.org/homerent/lastRenovationYear
:lastRenovationYear rdf:type owl:DatatypeProperty ;
                    rdfs:domain schema:Apartment ;
                    rdfs:range xsd:integer ;
                    rdfs:comment "Questa proprietà indica l'anno dell'ultima ristrotturazione."@it ,
                                 "This property indicates the last renovation year."@en ;
                    rdfs:isDefinedBy <https://purl.org/homerent/> ;
                    rdfs:label "anno dell'ultima ristrotturazione"@it ,
                               "last renovation year"@en .


###  https://purl.org/homerent/rentAdCode
:rentAdCode rdf:type owl:DatatypeProperty ,
                     owl:FunctionalProperty ;
            rdfs:range xsd:string ;
            rdfs:comment "Questa proprietà permette di specificare il codice dell'annuncio di affitto."@it ,
                         "This property allows to specify the rent ad code."@en ;
            rdfs:isDefinedBy <https://purl.org/homerent/> ;
            rdfs:label "codice dell'annuncio di affitto"@it ,
                       "rent ad code"@en .


###  https://purl.org/homerent/serviceDescription
:serviceDescription rdf:type owl:DatatypeProperty ;
                    rdfs:range xsd:string ;
                    rdfs:comment "Questa proprietà permette di descrivere un servizio messo a disposizione nell'appartamento."@it ,
                                 "This property allows to describe a service provided in the apartment."@en ;
                    rdfs:isDefinedBy <https://purl.org/homerent/> ;
                    rdfs:label "descrizione del servizio"@it ,
                               "service description"@en .


###  https://purl.org/homerent/totalPrice
:totalPrice rdf:type owl:DatatypeProperty ,
                     owl:FunctionalProperty ;
            rdfs:range xsd:float ;
            rdfs:comment "Questa proprietà permette di specificare il prezzo totale in un prezzo composto."@it ,
                         "This property allows to specify the total price in a compound price."@en ;
            rdfs:isDefinedBy <https://purl.org/homerent/> ;
            rdfs:label "prezzo totale"@it ,
                       "total price"@en .


#################################################################
#    Classes
#################################################################

###  http://purl.org/goodrelations/v1#UnitPriceSpecification
<http://purl.org/goodrelations/v1#UnitPriceSpecification> owl:equivalentClass [ rdf:type owl:Class ;
                                                                                owl:unionOf ( :ElectricityPrice
                                                                                              :HeatingPrice
                                                                                              :RentalPrice
                                                                                              :ServicePrice
                                                                                              :WaterPrice
                                                                                            )
                                                                              ] ;
                                                          rdfs:subClassOf [ rdf:type owl:Restriction ;
                                                                            owl:onProperty <http://purl.org/goodrelations/v1#hasCurrency> ;
                                                                            owl:someValuesFrom xsd:string
                                                                          ] ,
                                                                          [ rdf:type owl:Restriction ;
                                                                            owl:onProperty <http://purl.org/goodrelations/v1#hasCurrencyValue> ;
                                                                            owl:someValuesFrom xsd:float
                                                                          ] ,
                                                                          [ rdf:type owl:Restriction ;
                                                                            owl:onProperty <http://purl.org/goodrelations/v1#hasUnitOfMeasurement> ;
                                                                            owl:someValuesFrom xsd:string
                                                                          ] ,
                                                                          [ rdf:type owl:Restriction ;
                                                                            owl:onProperty <http://purl.org/goodrelations/v1#name> ;
                                                                            owl:someValuesFrom rdfs:Literal
                                                                          ] .


###  http://schema.org/Apartment
schema:Apartment rdf:type owl:Class .


###  http://schema.org/BusStop
schema:BusStop rdf:type owl:Class ;
               rdfs:subClassOf :PublicTransport ,
                               [ rdf:type owl:Restriction ;
                                 owl:onProperty :busLine ;
                                 owl:someValuesFrom xsd:string
                               ] ;
               owl:disjointWith schema:TrainStation .


###  http://schema.org/CollegeOrUniversity
schema:CollegeOrUniversity rdf:type owl:Class ;
                           rdfs:subClassOf :ReachablePlace .


###  http://schema.org/Event
schema:Event rdf:type owl:Class .


###  http://schema.org/ExerciseGym
schema:ExerciseGym rdf:type owl:Class ;
                   rdfs:subClassOf :ReachablePlace .


###  http://schema.org/Hospital
schema:Hospital rdf:type owl:Class ;
                rdfs:subClassOf :ReachablePlace .


###  http://schema.org/Museum
schema:Museum rdf:type owl:Class ;
              rdfs:subClassOf :ReachablePlace .


###  http://schema.org/Pharmacy
schema:Pharmacy rdf:type owl:Class ;
                rdfs:subClassOf :ReachablePlace .


###  http://schema.org/PostalAddress
schema:PostalAddress rdf:type owl:Class .


###  http://schema.org/TrainStation
schema:TrainStation rdf:type owl:Class ;
                    rdfs:subClassOf :PublicTransport .


###  http://xmlns.com/foaf/0.1/Person
foaf:Person rdf:type owl:Class .


###  https://purl.org/homerent/AirConditioner
:AirConditioner rdf:type owl:Class ;
                rdfs:subClassOf :Appliance ;
                rdfs:comment "Questa classe modella l'aria condizionata."@it ,
                             "This class models the air conditioner."@en ;
                rdfs:isDefinedBy <https://purl.org/homerent/> ;
                rdfs:label "Air conditioner"@en ,
                           "Aria condizionata"@it .


###  https://purl.org/homerent/Appliance
:Appliance rdf:type owl:Class ;
           rdfs:subClassOf :Feature ;
           owl:disjointWith :Service ;
           rdfs:comment "Questa classe funge da superclasse per gli elettrodomestici presenti nell'appartamento."@it ,
                        "This class act as a superclass for all the appliances inside the apartment."@en ;
           rdfs:isDefinedBy <https://purl.org/homerent/> ;
           rdfs:label "Appliance"@en ,
                      "Elettrodomestico"@it .


###  https://purl.org/homerent/Balcony
:Balcony rdf:type owl:Class ;
         rdfs:subClassOf :Service ;
         rdfs:comment "Questa classe modella la presenza di un balcone nell'appartamento"@it ,
                      "This class models the presence of a balcony in the apartment."@en ;
         rdfs:isDefinedBy <https://purl.org/homerent/> ;
         rdfs:label "Balcone"@it ,
                    "Balcony"@en .


###  https://purl.org/homerent/Bathroom
:Bathroom rdf:type owl:Class ;
          rdfs:subClassOf :Service ;
          rdfs:comment "Questa classe modella la presenza di un bagno"@it ,
                       "This class models the presence of a bathroom."@en ;
          rdfs:isDefinedBy <https://purl.org/homerent/> ;
          rdfs:label "Bagno"@it ,
                     "Bathroom"@en .


###  https://purl.org/homerent/BikeSharing
:BikeSharing rdf:type owl:Class ;
             rdfs:subClassOf :SharedMobility ;
             rdfs:comment "Questa classe modella il servizio di condivisione delle bici."@it ,
                          "This class models the bike sharing service."@en ;
             rdfs:isDefinedBy <https://purl.org/homerent/> ;
             rdfs:label "Bici in condivisione"@it ,
                        "Bike sharing"@en .


###  https://purl.org/homerent/CarSharing
:CarSharing rdf:type owl:Class ;
            rdfs:subClassOf :SharedMobility ;
            rdfs:comment "Questa classe modella il servizio di condivisione della macchina."@it ,
                         "This class models the service of car sharing."@en ;
            rdfs:isDefinedBy <https://purl.org/homerent/> ;
            rdfs:label "Car sharing"@en ,
                       "Macchina in condivisione"@it .


###  https://purl.org/homerent/CompoundPrice
:CompoundPrice rdf:type owl:Class ;
               rdfs:subClassOf <http://purl.org/goodrelations/v1#PriceSpecification> ,
                               :HomeRentEntity ,
                               [ rdf:type owl:Restriction ;
                                 owl:onProperty :priceComponent ;
                                 owl:someValuesFrom <http://purl.org/goodrelations/v1#UnitPriceSpecification>
                               ] ;
               rdfs:comment "A compound price specification is one that bundles multiple prices that all apply in combination for different dimensions of consumption."@en ,
                            "Una specifica di prezzo composto è quella che raggruppa più prezzi che si applicano tutti in combinazione per diverse dimensioni di consumo."@it ;
               rdfs:isDefinedBy <https://purl.org/homerent/> ;
               rdfs:label "Compound price"@en ,
                          "Prezzo composto"@it .


###  https://purl.org/homerent/Dishwasher
:Dishwasher rdf:type owl:Class ;
            rdfs:subClassOf :Appliance ;
            rdfs:comment "Questa classe modella una lavastoviglie utilizzabile all'interno dell'appartamento."@it ,
                         "This class models a dishwasher that can be used inside the apartment."@en ;
            rdfs:isDefinedBy <https://purl.org/homerent/> ;
            rdfs:label "Dishwasher"@en ,
                       "Lavastoviglie"@it .


###  https://purl.org/homerent/Dryer
:Dryer rdf:type owl:Class ;
       rdfs:subClassOf :Appliance ;
       rdfs:comment "Questa classe modella un'asciugatrice utilizzabile all'interno dell'appartamento."@it ,
                    "This class models a dryer that can be used inside the apartment."@en ;
       rdfs:isDefinedBy <https://purl.org/homerent/> ;
       rdfs:label "Asciugatrice"@it ,
                  "Dryer"@en .


###  https://purl.org/homerent/ElectricFan
:ElectricFan rdf:type owl:Class ;
             rdfs:subClassOf :Appliance ;
             rdfs:comment "Questa classe modella un ventilatore utilizzabile all'interno dell'appartamento."@it ,
                          "This class models an electric fan that can be used inside the apartment."@en ;
             rdfs:isDefinedBy <https://purl.org/homerent/> ;
             rdfs:label "Electric fan"@en ,
                        "Ventilatore"@it .


###  https://purl.org/homerent/ElectricityPrice
:ElectricityPrice rdf:type owl:Class ;
                  rdfs:subClassOf <http://purl.org/goodrelations/v1#UnitPriceSpecification> ,
                                  :HomeRentEntity ;
                  rdfs:comment "Questa specifica di prezzo descrive il prezzo per l'elettricità."@it ,
                               "This unit price specification describe the price for the electricity."@en ;
                  rdfs:isDefinedBy <https://purl.org/homerent/> ;
                  rdfs:label "Electricity price"@en ,
                             "Prezzo dell'elettricità"@it .


###  https://purl.org/homerent/Feature
:Feature rdf:type owl:Class ;
         owl:equivalentClass [ rdf:type owl:Class ;
                               owl:unionOf ( :Appliance
                                             :Service
                                           )
                             ] ;
         rdfs:subClassOf :HomeRentEntity ,
                         [ rdf:type owl:Restriction ;
                           owl:onProperty schema:description ;
                           owl:someValuesFrom xsd:string
                         ] ,
                         [ rdf:type owl:Restriction ;
                           owl:onProperty :isFeatureUsageShared ;
                           owl:someValuesFrom xsd:boolean
                         ] ;
         rdfs:comment "Questa classe funge da superclasse per tutte le caratteristiche che possono caratterizzare un appartamento."@it ,
                      "This class acts as a superclass for all characteristics that can characterize an apartment."@en ;
         rdfs:isDefinedBy <https://purl.org/homerent/> ;
         rdfs:label "Feature"@en ,
                    "Funzionalità"@it .


###  https://purl.org/homerent/FloorType
:FloorType rdf:type owl:Class ;
           owl:equivalentClass [ rdf:type owl:Class ;
                                 owl:oneOf ( :CeramicFloor
                                             :LaminateFloor
                                             :ParquetFloor
                                             :PorcelainStoneWareFloor
                                             :PvcFloor
                                             :ResinFloor
                                           )
                               ] ;
           rdfs:subClassOf :HomeRentEntity ;
           rdfs:comment "Questa classe modella il tipo di pavimentazione presente negli appartamenti."@it ,
                        "This class models the types of floor inside an apartment."@en ;
           rdfs:isDefinedBy <https://purl.org/homerent/> ;
           rdfs:label "Floor type"@en ,
                      "Tipo di pavimentazione"@it .


###  https://purl.org/homerent/Freezer
:Freezer rdf:type owl:Class ;
         rdfs:subClassOf :Appliance ;
         rdfs:comment "Questa classe modella un congelatore utilizzabile all'interno dell'appartamento."@it ,
                      "This class models a freezer that can be used inside the apartment."@en ;
         rdfs:isDefinedBy <https://purl.org/homerent/> ;
         rdfs:label "Congelatore"@it ,
                    "Freezer"@en .


###  https://purl.org/homerent/Fridge
:Fridge rdf:type owl:Class ;
        rdfs:subClassOf :Appliance ;
        rdfs:comment "Questa classe modella un frigo utilizzabile all'interno dell'appartamento."@it ,
                     "This class models a fridge that can be used inside the apartment."@en ;
        rdfs:isDefinedBy <https://purl.org/homerent/> ;
        rdfs:label "Fridge"@en ,
                   "Frigo"@it .


###  https://purl.org/homerent/Garden
:Garden rdf:type owl:Class ;
        rdfs:subClassOf :Service ;
        rdfs:comment "Questa classe modella la presenza di un giardino"@it ,
                     "This class models the presence of a garden."@en ;
        rdfs:isDefinedBy <https://purl.org/homerent/> ;
        rdfs:label "Garden"@en ,
                   "Giardino"@it .


###  https://purl.org/homerent/HeatingPrice
:HeatingPrice rdf:type owl:Class ;
              rdfs:subClassOf <http://purl.org/goodrelations/v1#UnitPriceSpecification> ,
                              :HomeRentEntity ;
              rdfs:comment "Questa specifica di prezzo descrive il prezzo per il riscaldamento."@it ,
                           "This unit price specification describe the price for the heating."@en ;
              rdfs:isDefinedBy <https://purl.org/homerent/> ;
              rdfs:label "Heating price"@en ,
                         "Prezzo del riscaldamento"@it .


###  https://purl.org/homerent/HomeRentEntity
:HomeRentEntity rdf:type owl:Class ;
                rdfs:comment "Questa classe include tutte le classi definite nell'ontologia HomeRent."@it ,
                             "This class includes all the classes defined under the HomeRent ontology."@en ;
                rdfs:isDefinedBy <https://purl.org/homerent/> .


###  https://purl.org/homerent/InternetAccess
:InternetAccess rdf:type owl:Class ;
                rdfs:subClassOf :Service ;
                rdfs:comment "Questa classe modella la presenza dell'accesso ad Internet"@it ,
                             "This class models the presence of the Internet access."@en ;
                rdfs:isDefinedBy <https://purl.org/homerent/> ;
                rdfs:label "Accesso ad Internet"@it ,
                           "Internet access"@en .


###  https://purl.org/homerent/Kitchen
:Kitchen rdf:type owl:Class ;
         rdfs:subClassOf :Service ;
         rdfs:comment "Questa classe modella la presenza di una cucina"@it ,
                      "This class models the presence of a kitchen."@en ;
         rdfs:isDefinedBy <https://purl.org/homerent/> ;
         rdfs:label "Cucina"@it ,
                    "Kitchen"@en .


###  https://purl.org/homerent/Lift
:Lift rdf:type owl:Class ;
      rdfs:subClassOf :Service ;
      rdfs:comment "Questa classe modella la presenza di un ascensore"@it ,
                   "This class models the presence of a lift."@en ;
      rdfs:isDefinedBy <https://purl.org/homerent/> ;
      rdfs:label "Ascensore"@it ,
                 "Lift"@en .


###  https://purl.org/homerent/Microwave
:Microwave rdf:type owl:Class ;
           rdfs:subClassOf :Appliance ;
           rdfs:comment "Questa classe modella un microonde utilizzabile all'interno dell'appartamento."@it ,
                        "This class models a microwave that can be used inside the apartment."@en ;
           rdfs:isDefinedBy <https://purl.org/homerent/> ;
           rdfs:label "Microonde"@it ,
                      "Microwave"@en .


###  https://purl.org/homerent/Oven
:Oven rdf:type owl:Class ;
      rdfs:subClassOf :Appliance ;
      rdfs:comment "Questa classe modella un forno utilizzabile all'interno dell'appartamento."@it ,
                   "This class models an oven that can be used inside the apartment."@en ;
      rdfs:isDefinedBy <https://purl.org/homerent/> ;
      rdfs:label "Forno"@it ,
                 "Oven"@en .


###  https://purl.org/homerent/ParkingSpace
:ParkingSpace rdf:type owl:Class ;
              rdfs:subClassOf :Service ;
              rdfs:comment "Questa classe modella la presenza di uno spazio per il parcheggio"@it ,
                           "This class models the presence of a parking space."@en ;
              rdfs:isDefinedBy <https://purl.org/homerent/> ;
              rdfs:label "Parking space"@en ,
                         "Spazio per parcheggio"@it .


###  https://purl.org/homerent/PublicTransport
:PublicTransport rdf:type owl:Class ;
                 rdfs:subClassOf :ReachablePlace ;
                 rdfs:comment "Questa classe funge da superclasse per i servizi di trasporto pubblico."@it ,
                              "This class acts as a superclass for the public transport services."@en ;
                 rdfs:isDefinedBy <https://purl.org/homerent/> ;
                 rdfs:label "Public transport"@en ,
                            "Trasporto pubblico"@it .


###  https://purl.org/homerent/ReachablePlace
:ReachablePlace rdf:type owl:Class ;
                rdfs:subClassOf :HomeRentEntity ;
                rdfs:comment "Questa classe modella un luogo nella città."@it ,
                             "This class models a place inside the city."@en ;
                rdfs:isDefinedBy <https://purl.org/homerent/> ;
                rdfs:label "Luogo raggiungibile"@it ,
                           "Reachable place"@en .


###  https://purl.org/homerent/RentalAd
:RentalAd rdf:type owl:Class ;
          rdfs:subClassOf <http://purl.org/goodrelations/v1#Offering> ,
                          :HomeRentEntity ,
                          [ rdf:type owl:Restriction ;
                            owl:onProperty :isOfferedBy ;
                            owl:someValuesFrom <http://purl.org/goodrelations/v1#BusinessEntity>
                          ] ,
                          [ rdf:type owl:Restriction ;
                            owl:onProperty <http://purl.org/goodrelations/v1#includes> ;
                            owl:allValuesFrom schema:Apartment
                          ] ,
                          [ rdf:type owl:Restriction ;
                            owl:onProperty <http://purl.org/goodrelations/v1#hasPriceSpecification> ;
                            owl:cardinality "1"^^xsd:nonNegativeInteger
                          ] ,
                          [ rdf:type owl:Restriction ;
                            owl:onProperty <http://purl.org/goodrelations/v1#includes> ;
                            owl:qualifiedCardinality "1"^^xsd:nonNegativeInteger ;
                            owl:onClass schema:Apartment
                          ] ;
          owl:hasKey ( :rentAdCode
                     ) ;
          rdfs:comment "Questa classe modella un annuncio di affitto."@it ,
                       "This class models a rent ad."@en ;
          rdfs:isDefinedBy <https://purl.org/homerent/> ;
          rdfs:label "Annuncio di affitto"@it ,
                     "Rental Ad"@en .


###  https://purl.org/homerent/RentalAdInterest
:RentalAdInterest rdf:type owl:Class ;
                  rdfs:subClassOf schema:Event ,
                                  :HomeRentEntity ,
                                  [ rdf:type owl:Restriction ;
                                    owl:onProperty :isOfInterestTo ;
                                    owl:someValuesFrom schema:Person
                                  ] ,
                                  [ rdf:type owl:Restriction ;
                                    owl:onProperty :refersRentAd ;
                                    owl:someValuesFrom :RentalAd
                                  ] ,
                                  [ rdf:type owl:Restriction ;
                                    owl:onProperty :interestDateTime ;
                                    owl:someValuesFrom xsd:dateTime
                                  ] ;
                  rdfs:comment "Questa classe modella l'interesse in un annuncio di un affitto."@it ,
                               "This class models the interest in a rent ad."@en ;
                  rdfs:isDefinedBy <https://purl.org/homerent/> ;
                  rdfs:label "Interesse in un annuncio di affitto"@it ,
                             "Rental Ad Interest"@en .


###  https://purl.org/homerent/RentalPrice
:RentalPrice rdf:type owl:Class ;
             rdfs:subClassOf <http://purl.org/goodrelations/v1#UnitPriceSpecification> ,
                             :HomeRentEntity ;
             rdfs:comment "Questa specifica di prezzo descrive il prezzo per l'affitto dell'appartamento."@it ,
                          "This unit price specification describe the price for the rent."@en ;
             rdfs:isDefinedBy <https://purl.org/homerent/> ;
             rdfs:label "Prezzo di affitto"@it ,
                        "Rental Price"@en .


###  https://purl.org/homerent/ScooterSharing
:ScooterSharing rdf:type owl:Class ;
                rdfs:subClassOf :SharedMobility ;
                rdfs:comment "Questa classe modella il servizio di condivisione dei monopattini."@it ,
                             "This class models the scooter sharing service."@en ;
                rdfs:isDefinedBy <https://purl.org/homerent/> ;
                rdfs:label "Monopattini in condivisione"@it ,
                           "Scooter sharing"@en .


###  https://purl.org/homerent/Service
:Service rdf:type owl:Class ;
         rdfs:subClassOf :Feature ;
         rdfs:comment "Questa classe funge da superclasse per i servizi inclusi nell'appartamento."@it ,
                      "This class act as a superclass for the services included with the apartment."@en ;
         rdfs:isDefinedBy <https://purl.org/homerent/> ;
         rdfs:label "Service"@en ,
                    "Servizio"@it .


###  https://purl.org/homerent/ServicePrice
:ServicePrice rdf:type owl:Class ;
              rdfs:subClassOf <http://purl.org/goodrelations/v1#UnitPriceSpecification> ,
                              :HomeRentEntity ,
                              [ rdf:type owl:Restriction ;
                                owl:onProperty :serviceDescription ;
                                owl:someValuesFrom xsd:string
                              ] ;
              rdfs:comment "Questa specifica di prezzo descrive il prezzo per un servizio generale."@it ,
                           "This unit price specification describe the price for a general service."@en ;
              rdfs:isDefinedBy <https://purl.org/homerent/> ;
              rdfs:label "Prezzo del servizio"@it ,
                         "Service price"@en .


###  https://purl.org/homerent/SharedMobility
:SharedMobility rdf:type owl:Class ;
                rdfs:subClassOf :ReachablePlace ;
                rdfs:comment "Questa classe funge da superclasse per i servizi di mobilità condivisa."@it ,
                             "This class acts as a superclass for the shared mobility services."@en ;
                rdfs:isDefinedBy <https://purl.org/homerent/> ;
                rdfs:label "Mobilità condivisa"@it ,
                           "Shared mobility"@en .


###  https://purl.org/homerent/Stove
:Stove rdf:type owl:Class ;
       rdfs:subClassOf :Appliance ;
       rdfs:comment "Questa classe modella un piano cottura utilizzabile all'interno dell'appartamento."@it ,
                    "This class models a stove that can be used inside the apartment."@en ;
       rdfs:isDefinedBy <https://purl.org/homerent/> ;
       rdfs:label "Piano cottura"@it ,
                  "Stove"@en .


###  https://purl.org/homerent/StrategicPoint
:StrategicPoint rdf:type owl:Class ;
                rdfs:subClassOf :HomeRentEntity ,
                                [ rdf:type owl:Restriction ;
                                  owl:onProperty :reachableFrom ;
                                  owl:someValuesFrom schema:Apartment
                                ] ,
                                [ rdf:type owl:Restriction ;
                                  owl:onProperty :strategicPointRefersTo ;
                                  owl:someValuesFrom :ReachablePlace
                                ] ,
                                [ rdf:type owl:Restriction ;
                                  owl:onProperty :distanceInKm ;
                                  owl:someValuesFrom xsd:float
                                ] ;
                rdfs:comment "Questa classe modella un punto strategico che può essere raggiunto dall'appartamento."@it ,
                             "This class models a strategic point that can be reached from the apartment."@en ;
                rdfs:isDefinedBy <https://purl.org/homerent/> ;
                rdfs:label "Punto strategico"@it ,
                           "Strategic point"@en .


###  https://purl.org/homerent/Supermarket
:Supermarket rdf:type owl:Class ;
             rdfs:subClassOf :ReachablePlace ;
             rdfs:comment "Questa class modella un supermercato."@it ,
                          "This class models a supermarket."@en ;
             rdfs:isDefinedBy <https://purl.org/homerent/> ;
             rdfs:label "Supermarket"@en ,
                        "Supermercato"@it .


###  https://purl.org/homerent/TV
:TV rdf:type owl:Class ;
    rdfs:subClassOf :Appliance ;
    rdfs:comment "Questa classe modella una tv utilizzabile all'interno dell'appartamento."@it ,
                 "This class models a tv that can be used inside the apartment."@en ;
    rdfs:isDefinedBy <https://purl.org/homerent/> ;
    rdfs:label "TV"@en ,
               "TV"@it .


###  https://purl.org/homerent/Vacuum
:Vacuum rdf:type owl:Class ;
        rdfs:subClassOf :Appliance ;
        rdfs:comment "Questa classe modella un'aspirapolvere utilizzabile all'interno dell'appartamento."@it ,
                     "This class models a vacuum that can be used inside the apartment."@en ;
        rdfs:isDefinedBy <https://purl.org/homerent/> ;
        rdfs:label "Aspirapolvere"@it ,
                   "Vacuum"@en .


###  https://purl.org/homerent/WashingMachine
:WashingMachine rdf:type owl:Class ;
                rdfs:subClassOf :Appliance ;
                rdfs:comment "Questa classe modella una lavatrice utilizzabile all'interno dell'appartamento."@it ,
                             "This class models a washing machine that can be used inside the apartment."@en ;
                rdfs:isDefinedBy <https://purl.org/homerent/> ;
                rdfs:label "Lavatrice"@it ,
                           "Washing machine"@en .


###  https://purl.org/homerent/WaterPrice
:WaterPrice rdf:type owl:Class ;
            rdfs:subClassOf <http://purl.org/goodrelations/v1#UnitPriceSpecification> ,
                            :HomeRentEntity ;
            rdfs:comment "Questa specifica di prezzo descrive il prezzo per l'acqua."@it ,
                         "This unit price specification describe the price for the water."@en ;
            rdfs:isDefinedBy <https://purl.org/homerent/> ;
            rdfs:label "Prezzo dell'acqua"@it ,
                       "Water price"@en .


###  https://www.geonames.org/ontology#Feature
gn:Feature rdf:type owl:Class .


#################################################################
#    Individuals
#################################################################

###  https://purl.org/homerent/CeramicFloor
:CeramicFloor rdf:type owl:NamedIndividual ,
                       :FloorType ;
              :floorDescription """Ceramic floor tiles are durable, versatile, and aesthetically pleasing flooring materials made from clay and other natural substances.
They come in a variety of colors, patterns, and textures, allowing for numerous design options to suit different styles and preferences.
Ceramic tiles are highly resistant to wear, moisture, and stains, making them suitable for high-traffic areas and easy to maintain with regular cleaning."""@en .


###  https://purl.org/homerent/LaminateFloor
:LaminateFloor rdf:type owl:NamedIndividual ,
                        :FloorType ;
               :floorDescription "Laminate flooring (also called floating wood tile in the United States) is a multi-layer synthetic flooring product fused together with a lamination process. Laminate flooring simulates wood (or sometimes stone) with a photographic applique layer under a clear protective layer."@en .


###  https://purl.org/homerent/ParquetFloor
:ParquetFloor rdf:type owl:NamedIndividual ,
                       :FloorType ;
              :floorDescription "Parquet is a type of wood flooring made by arranging small slats of wood in distinct, repeating patterns. While traditional parquet floors were installed one piece at a time, most modern parquet comes in tile form in which the wood slats are bonded to a backing material."@en .


###  https://purl.org/homerent/PorcelainStoneWareFloor
:PorcelainStoneWareFloor rdf:type owl:NamedIndividual ,
                                  :FloorType ;
                         :floorDescription """Porcelain stoneware floor is a type of ceramic tile that is extremely dense and durable, made from a specific type of clay fired at very high temperatures.
It is highly resistant to wear, scratches, stains, and moisture, making it suitable for both indoor and outdoor use, including high-traffic areas and areas prone to water exposure such as bathrooms and kitchens.
Porcelain stoneware floor tiles come in a wide variety of colors, finishes, and sizes, and can replicate the look of natural materials such as stone, concrete, or wood. They offer a combination of aesthetic appeal and practicality, making them a popular choice for residential and commercial spaces."""@en .


###  https://purl.org/homerent/PvcFloor
:PvcFloor rdf:type owl:NamedIndividual ,
                   :FloorType ;
          :floorDescription """PVC flooring is a type of flooring made from polyvinyl chloride, a synthetic plastic.
It is moisture-resistant, scratch-resistant, and stain-resistant, making it a good choice for high-traffic areas.
PVC flooring is available in a variety of colors, patterns, and textures, making it a versatile option for any home."""@en .


###  https://purl.org/homerent/ResinFloor
:ResinFloor rdf:type owl:NamedIndividual ,
                     :FloorType ;
            :floorDescription """Resin flooring is a type of flooring made from epoxy resin or polyurethane resin.
It is durable, water-resistant, and chemical-resistant, making it a good choice for high-traffic areas.
Resin flooring is available in a variety of colors, patterns, and textures, making it a versatile option for any home."""@en .


#################################################################
#    General axioms
#################################################################

[ rdf:type owl:AllDisjointClasses ;
  owl:members ( schema:CollegeOrUniversity
                schema:ExerciseGym
                schema:Hospital
                schema:Museum
                schema:Pharmacy
                :PublicTransport
                :SharedMobility
                :Supermarket
              )
] .


[ rdf:type owl:AllDisjointClasses ;
  owl:members ( :AirConditioner
                :Dishwasher
                :Dryer
                :ElectricFan
                :Freezer
                :Fridge
                :Microwave
                :Oven
                :Stove
                :TV
                :Vacuum
                :WashingMachine
              )
] .


[ rdf:type owl:AllDisjointClasses ;
  owl:members ( :Balcony
                :Bathroom
                :Garden
                :InternetAccess
                :Kitchen
                :Lift
                :ParkingSpace
              )
] .


[ rdf:type owl:AllDisjointClasses ;
  owl:members ( :BikeSharing
                :CarSharing
                :ScooterSharing
              )
] .


[ rdf:type owl:AllDisjointClasses ;
  owl:members ( :CompoundPrice
                :ElectricityPrice
                :Feature
                :FloorType
                :HeatingPrice
                :ReachablePlace
                :RentalAd
                :RentalAdInterest
                :RentalPrice
                :ServicePrice
                :StrategicPoint
                :WaterPrice
              )
] .


###  Generated by the OWL API (version 4.5.25.2023-02-15T19:15:49Z) https://github.com/owlcs/owlapi
